

Solutions

Problem 1 (Convex functions and convex sets)

- (a) **i) Polyhedron.** Let $P = \{x \in \mathbb{R}^n \mid Ax \leq b\}$ (componentwise). Take any $x_1, x_2 \in P$ and any $\theta \in [0, 1]$. Then

$$A(\theta x_1 + (1 - \theta)x_2) = \theta Ax_1 + (1 - \theta)Ax_2 \leq \theta b + (1 - \theta)b = b.$$

Hence $\theta x_1 + (1 - \theta)x_2 \in P$, so P is convex.

- ii) ℓ_1 -ball.** Let $B_1(r) = \{x \in \mathbb{R}^n : \|x\|_1 \leq r\}$. For any $x_1, x_2 \in B_1(r)$ and $\theta \in [0, 1]$, by triangle inequality and homogeneity of $\|\cdot\|_1$,

$$\|\theta x_1 + (1 - \theta)x_2\|_1 \leq \|\theta x_1\|_1 + \|(1 - \theta)x_2\|_1 = \theta\|x_1\|_1 + (1 - \theta)\|x_2\|_1 \leq r.$$

So $B_1(r)$ is convex.

- iii) PSD cone.** Let $S_+^n = \{X \in S^n : X \succeq 0\}$. Take $X, Y \succeq 0$ and $\theta \in [0, 1]$. For any $v \in \mathbb{R}^n$,

$$v^\top(\theta X + (1 - \theta)Y)v = \theta v^\top X v + (1 - \theta)v^\top Y v \geq 0.$$

Thus $\theta X + (1 - \theta)Y \succeq 0$ and S_+^n is convex.

- (b) **i) $f(x) = \|x\|_1$ is convex.** For any $x_1, x_2 \in \mathbb{R}^n$ and $\theta \in [0, 1]$,

$$\|\theta x_1 + (1 - \theta)x_2\|_1 \leq \theta\|x_1\|_1 + (1 - \theta)\|x_2\|_1,$$

by the same argument as in (a-ii). Hence f is convex.

- ii) If f, g are convex, then $f + g$ is convex.** For any x_1, x_2 and $\theta \in [0, 1]$,

$$\begin{aligned} (f + g)(\theta x_1 + (1 - \theta)x_2) &= f(\theta x_1 + (1 - \theta)x_2) + g(\theta x_1 + (1 - \theta)x_2) \\ &\leq \theta f(x_1) + (1 - \theta)f(x_2) + \theta g(x_1) + (1 - \theta)g(x_2) \\ &= \theta(f + g)(x_1) + (1 - \theta)(f + g)(x_2). \end{aligned}$$

- iii) A counterexample for composition.** Let outer $f(u) = -u$ (affine, hence convex) and inner $g(x) = x^2$ (convex). Then $(f \circ g)(x) = -x^2$, which is *not* convex. So composition of convex functions is not always convex.

Problem 2 (Strong Convexity)

A differentiable function is μ -strongly convex if

$$f(y) \geq f(x) + \langle \nabla f(x), y - x \rangle + \frac{\mu}{2}\|y - x\|_2^2, \quad \forall x, y.$$

- (a) Let x^* be a minimizer of f . Since f is differentiable and convex, $\nabla f(x^*) = 0$. Apply strong convexity with $x = x^*$, $y = x$:

$$f(x) \geq f(x^*) + \langle \nabla f(x^*), x - x^* \rangle + \frac{\mu}{2} \|x - x^*\|_2^2 = f(x^*) + \frac{\mu}{2} \|x - x^*\|_2^2,$$

$$\text{hence } f(x) - f(x^*) \geq \frac{\mu}{2} \|x - x^*\|_2^2.$$

- (b) For $f(x) = \frac{1}{2}x^\top Ax + b^\top x$, the Hessian is A . The largest valid μ equals $\lambda_{\min}(A)$. Given

$$A = \begin{pmatrix} 6 & 2 \\ 2 & 9 \end{pmatrix},$$

its eigenvalues satisfy $\lambda^2 - \text{tr}(A)\lambda + \det(A) = 0$:

$$\lambda^2 - 15\lambda + 50 = 0 \Rightarrow \lambda = \frac{15 \pm \sqrt{225 - 200}}{2} = \frac{15 \pm 5}{2} \in \{10, 5\}.$$

Thus $\mu_{\max} = \lambda_{\min}(A) = 5$.

Problem 3 (Prox operators for ℓ_0 and ℓ_2)

- (a) $\text{prox}_{\lambda\|\cdot\|_0}(v)$. Recall $\|x\|_0 = \sum_{i=1}^n \mathbf{1}(x_i \neq 0)$. The objective is separable:

$$\begin{aligned} \text{prox}_{\lambda\|\cdot\|_0}(v) &= \arg \min_{x \in \mathbb{R}^n} \left\{ \lambda \|x\|_0 + \frac{1}{2} \|x - v\|_2^2 \right\} \\ &= \left(\arg \min_{x_i \in \mathbb{R}} \{ \lambda \mathbf{1}(x_i \neq 0) + \frac{1}{2} (x_i - v_i)^2 \} \right)_{i=1}^n. \end{aligned}$$

Fix coordinate i . Consider two cases:

$$\text{If } x_i = 0: \quad \lambda \mathbf{1}(x_i \neq 0) + \frac{1}{2} (x_i - v_i)^2 = \frac{1}{2} v_i^2.$$

$$\text{If } x_i \neq 0: \quad \lambda + \frac{1}{2} (x_i - v_i)^2 \text{ is minimized at } x_i = v_i, \text{ giving value } \lambda.$$

Hence we choose $x_i = v_i$ if $\lambda < \frac{1}{2} v_i^2$, i.e., $|v_i| > \sqrt{2\lambda}$, and choose $x_i = 0$ if $\lambda > \frac{1}{2} v_i^2$, i.e., $|v_i| < \sqrt{2\lambda}$. At the tie $|v_i| = \sqrt{2\lambda}$, both 0 and v_i are minimizers. Therefore,

$$(\text{prox}_{\lambda\|\cdot\|_0}(v))_i \in \begin{cases} \{v_i\}, & |v_i| > \sqrt{2\lambda}, \\ \{0, v_i\}, & |v_i| = \sqrt{2\lambda}, \\ \{0\}, & |v_i| < \sqrt{2\lambda}. \end{cases}$$

Equivalently (choosing the common convention that breaks ties by 0), this is the hard-thresholding rule

$$(\text{prox}_{\lambda\|\cdot\|_0}(v))_i = \begin{cases} v_i, & |v_i| > \sqrt{2\lambda}, \\ 0, & |v_i| \leq \sqrt{2\lambda}. \end{cases}$$

(b) $\text{prox}_{\lambda\|\cdot\|_2}(v)$. We solve

$$\text{prox}_{\lambda\|\cdot\|_2}(v) = \arg \min_{x \in \mathbb{R}^n} \left\{ \lambda \|x\|_2 + \frac{1}{2} \|x - v\|_2^2 \right\}.$$

Write $x = ru$ where $r = \|x\|_2 \geq 0$ and $\|u\|_2 = 1$ (for $x \neq 0$). Then

$$\|x - v\|_2^2 = \|ru - v\|_2^2 = r^2 - 2r\langle u, v \rangle + \|v\|_2^2.$$

For fixed r , minimizing over $\|u\|_2 = 1$ is equivalent to maximizing $\langle u, v \rangle$, achieved by $u = \frac{v}{\|v\|_2}$ when $v \neq 0$, giving $\max \langle u, v \rangle = \|v\|_2$. Thus the problem reduces to

$$\min_{r \geq 0} \lambda r + \frac{1}{2} (r - \|v\|_2)^2 \quad (\text{up to an additive constant } \frac{1}{2} \|v\|_2^2).$$

Solve this quadratic problem coordinate by coordinate we can get

$$r^* = \max(\|v\|_2 - \lambda, 0).$$

Hence, for $v \neq 0$,

$$x^* = r^* \frac{v}{\|v\|_2} = \begin{cases} \left(1 - \frac{\lambda}{\|v\|_2}\right) v, & \|v\|_2 > \lambda, \\ 0, & \|v\|_2 \leq \lambda. \end{cases}$$

This is the vector (group) soft-thresholding / shrinkage operator:

$$\text{prox}_{\lambda\|\cdot\|_2}(v) = \left(1 - \frac{\lambda}{\|v\|_2}\right)_+ v, \quad \text{where } (t)_+ = \max(t, 0),$$

and the formula also yields 0 when $v = 0$.

(c) Compute three proximal operators for $\lambda = 1$.

Let $v^{(1)} = (1, 1)$ and $v^{(2)} = (2, 0)$, with $\lambda = 1$ so $\sqrt{2\lambda} = \sqrt{2}$.

$$\begin{aligned} \text{prox}_{\|\cdot\|_0}(v^{(1)}) &= (0, 0) \quad \text{since } |1| \leq \sqrt{2} \text{ for both coordinates,} \\ \text{prox}_{\|\cdot\|_0}(v^{(2)}) &= (2, 0) \quad \text{since } |2| > \sqrt{2}, |0| \leq \sqrt{2}. \end{aligned}$$

$$\begin{aligned} \text{prox}_{\|\cdot\|_1}(v^{(1)}) &= (\max(1 - 1, 0), \max(1 - 1, 0)) = (0, 0), \\ \text{prox}_{\|\cdot\|_1}(v^{(2)}) &= (\max(2 - 1, 0), 0) = (1, 0). \end{aligned}$$

$$\begin{aligned} \text{prox}_{\|\cdot\|_2}(v^{(1)}) &= \left(1 - \frac{1}{\|(1, 1)\|_2}\right) (1, 1) = \left(1 - \frac{1}{\sqrt{2}}\right) (1, 1), \\ \text{prox}_{\|\cdot\|_2}(v^{(2)}) &= \left(1 - \frac{1}{\|(2, 0)\|_2}\right) (2, 0) = \left(1 - \frac{1}{2}\right) (2, 0) = (1, 0). \end{aligned}$$

Problem 4 (Convergence of Projected Gradient Descent)

(a) Since f is L -smooth, for all x, y we have the descent lemma

$$f(y) \leq f(x) + \langle \nabla f(x), y - x \rangle + \frac{L}{2} \|y - x\|^2.$$

Taking $x = x_k$ and $y = x_{k+1}$ gives

$$f(x_{k+1}) \leq f(x_k) + \langle \nabla f(x_k), x_{k+1} - x_k \rangle + \frac{L}{2} \|x_{k+1} - x_k\|^2.$$

Adding $g(x_{k+1})$ to both sides and using the definition of $Q_L(\cdot; x_k)$ yields

$$F(x_{k+1}) = f(x_{k+1}) + g(x_{k+1}) \leq Q_L(x_{k+1}; x_k).$$

(b) The function $x \mapsto \frac{L}{2} \|x - x_k\|^2$ is L -strongly convex, the term $x \mapsto f(x_k) + \langle \nabla f(x_k), x - x_k \rangle$ is affine (hence convex), and g is convex. Therefore their sum $Q_L(\cdot; x_k)$ is L -strongly convex.

Let $x_{k+1} = \arg \min_x Q_L(x; x_k)$. A standard consequence of μ -strong convexity (with $\mu = L$) is: for all x ,

$$Q_L(x; x_k) \geq Q_L(x_{k+1}; x_k) + \frac{L}{2} \|x - x_{k+1}\|^2.$$

This is exactly the desired inequality.

(c) From (a) and (b), for any $x \in \mathbb{R}^n$,

$$F(x_{k+1}) \leq Q_L(x_{k+1}; x_k) \leq Q_L(x; x_k) - \frac{L}{2} \|x - x_{k+1}\|^2,$$

hence

$$F(x_{k+1}) \leq Q_L(x; x_k) - \frac{L}{2} \|x - x_{k+1}\|^2, \quad \forall x.$$

Next, by convexity of f ,

$$f(x) \geq f(x_k) + \langle \nabla f(x_k), x - x_k \rangle,$$

so

$$\begin{aligned} Q_L(x; x_k) &= f(x_k) + \langle \nabla f(x_k), x - x_k \rangle + \frac{L}{2} \|x - x_k\|^2 + g(x) \\ &\leq f(x) + g(x) + \frac{L}{2} \|x - x_k\|^2 \\ &= F(x) + \frac{L}{2} \|x - x_k\|^2. \end{aligned}$$

Substituting this bound into the previous inequality yields the key estimate:

$$F(x_{k+1}) \leq F(x) + \frac{L}{2} \left(\|x - x_k\|^2 - \|x - x_{k+1}\|^2 \right), \quad \forall x.$$

- (d) Let $x^\star \in X^\star$ be any minimizer, and denote $F^\star = F(x^\star) = \min_x F(x)$. Applying the key estimate in (c) with $x = x^\star$ gives, for all k ,

$$F(x_{k+1}) - F^\star \leq \frac{L}{2} \left(\|x^\star - x_k\|^2 - \|x^\star - x_{k+1}\|^2 \right).$$

Summing from $k = 0$ to $K - 1$ (telescoping) yields

$$\sum_{k=0}^{K-1} (F(x_{k+1}) - F^\star) \leq \frac{L}{2} \left(\|x^\star - x_0\|^2 - \|x^\star - x_K\|^2 \right) \leq \frac{L}{2} \|x_0 - x^\star\|^2.$$

Moreover, choosing $x = x_k$ in (c) gives monotonic decrease:

$$F(x_{k+1}) \leq F(x_k), \quad \forall k,$$

so $F(x_K) \leq F(x_k)$ for all $k \leq K$, and hence

$$F(x_K) - F^\star \leq \frac{1}{K} \sum_{k=0}^{K-1} (F(x_{k+1}) - F^\star) \leq \frac{L}{2K} \|x_0 - x^\star\|^2.$$

This proves the $O(1/K)$ convergence rate of objective values.

Problem 5 (Backtracking when L is unknown)

Backtracking rule: accept \hat{L} if

$$f\left(x - \frac{1}{\hat{L}} \nabla f(x)\right) \leq f(x) - \frac{1}{2\hat{L}} \|\nabla f(x)\|_2^2.$$

- (a) Let $y = x - \frac{1}{\hat{L}} \nabla f(x)$. By descent lemma (with true L),

$$f(y) \leq f(x) + \langle \nabla f(x), y - x \rangle + \frac{L}{2} \|y - x\|_2^2.$$

Here $y - x = -\frac{1}{\hat{L}} \nabla f(x)$, so

$$f(y) \leq f(x) - \frac{1}{\hat{L}} \|\nabla f(x)\|_2^2 + \frac{L}{2} \cdot \frac{1}{\hat{L}^2} \|\nabla f(x)\|_2^2 = f(x) - \left(\frac{1}{\hat{L}} - \frac{L}{2\hat{L}^2} \right) \|\nabla f(x)\|_2^2.$$

If $\hat{L} \geq L$, then

$$\frac{1}{\hat{L}} - \frac{L}{2\hat{L}^2} = \frac{1}{2\hat{L}} \left(2 - \frac{L}{\hat{L}} \right) \geq \frac{1}{2\hat{L}},$$

hence

$$f\left(x - \frac{1}{\hat{L}} \nabla f(x)\right) \leq f(x) - \frac{1}{2\hat{L}} \|\nabla f(x)\|_2^2.$$

Therefore any $\hat{L} \geq L$ will be accepted, so the loop terminates in finitely many trials.

- (b) Starting from $\hat{L} = \hat{L}_k$, after N multiplications the trial value is $\hat{L}_k \eta^N$. The loop must accept once $\hat{L}_k \eta^N \geq L$. Thus the smallest such N satisfies

$$N \leq \left\lceil \log_\eta \left(\frac{L}{\hat{L}_k} \right) \right\rceil_+, \quad \text{where } [t]_+ = \max\{0, [t]\}.$$

Problem 6 (APGD objective is not necessarily monotone)

APGD update:

$$y_k = x_k + \beta(x_k - x_{k-1}), \quad x_{k+1} = y_k - \alpha \nabla f(y_k).$$

Take $f(x) = \frac{1}{2}x^2$, $\nabla f(x) = x$, $\alpha = \frac{1}{2}$, $\beta = 4$, and $x_{-1} = x_0 = 1$.

(a) First step:

$$y_0 = x_0 + 4(x_0 - x_{-1}) = 1, \quad x_1 = y_0 - \frac{1}{2}y_0 = \frac{1}{2}.$$

Second step:

$$\begin{aligned} y_1 &= x_1 + 4(x_1 - x_0) = \frac{1}{2} + 4\left(\frac{1}{2} - 1\right) = \frac{1}{2} - 2 = -\frac{3}{2}, \\ x_2 &= y_1 - \frac{1}{2}y_1 = \frac{1}{2}y_1 = -\frac{3}{4}. \end{aligned}$$

Compute objective values:

$$f(x_1) = \frac{1}{2} \left(\frac{1}{2}\right)^2 = \frac{1}{8}, \quad f(x_2) = \frac{1}{2} \left(\frac{3}{4}\right)^2 = \frac{9}{32}.$$

Since $\frac{9}{32} > \frac{1}{8}$, the objective increases, so APGD is not necessarily monotone.

(b) The extrapolation $y_k = x_k + \beta(x_k - x_{k-1})$ adds “momentum” in the recent moving direction. If β is large, y_k can jump past the minimizer (overshoot), so the next gradient step may land at a point with a larger function value.